refactor(library/init/data/array): new name convention for Array functions

library/init/data/array/basic.lean
@@ -65,7 +65,7 @@ def singleton (v : α) : Array α :=
 mkArray 1 v
 
 @[extern c inline "lean_array_fget(#2, #3)"]
-def fget (a : @& Array α) (i : @& Fin a.size) : α :=
+def get (a : @& Array α) (i : @& Fin a.size) : α :=
 a.data i
 
 /- Low-level version of `fget` which is as fast as a C array read.
@@ -73,25 +73,25 @@ a.data i
    `fget` may be slightly slower than `uget`. -/
 @[extern c inline "lean_array_uget(#2, #3)"]
 def uget (a : @& Array α) (i : USize) (h : i.toNat < a.size) : α :=
-a.fget ⟨i.toNat, h⟩
+a.get ⟨i.toNat, h⟩
 
 /- "Comfortable" version of `fget`. It performs a bound check at runtime. -/
 @[extern c inline "lean_array_get(#2, #3, #4)"]
-def get [Inhabited α] (a : @& Array α) (i : @& Nat) : α :=
-if h : i < a.size then a.fget ⟨i, h⟩ else default α
+def get! [Inhabited α] (a : @& Array α) (i : @& Nat) : α :=
+if h : i < a.size then a.get ⟨i, h⟩ else default α
 
 def back [Inhabited α] (a : Array α) : α :=
-a.get (a.size - 1)
+a.get! (a.size - 1)
 
-def getOpt (a : Array α) (i : Nat) : Option α :=
-if h : i < a.size then some (a.fget ⟨i, h⟩) else none
+def get? (a : Array α) (i : Nat) : Option α :=
+if h : i < a.size then some (a.get ⟨i, h⟩) else none
 
 @[extern c inline "lean_array_fset(#2, #3, #4)"]
-def fset (a : Array α) (i : @& Fin a.size) (v : α) : Array α :=
+def set (a : Array α) (i : @& Fin a.size) (v : α) : Array α :=
 { sz   := a.sz,
   data := fun j => if h : i = j then v else a.data j }
 
-theorem szFSetEq (a : Array α) (i : Fin a.size) (v : α) : (fset a i v).size = a.size :=
+theorem szFSetEq (a : Array α) (i : Fin a.size) (v : α) : (set a i v).size = a.size :=
 rfl
 
 theorem szPushEq (a : Array α) (v : α) : (push a v).size = a.size + 1 :=
@@ -102,39 +102,43 @@ rfl
    `fset` may be slightly slower than `uset`. -/
 @[extern c inline "lean_array_uset(#2, #3, #4)"]
 def uset (a : Array α) (i : USize) (v : α) (h : i.toNat < a.size) : Array α :=
-a.fset ⟨i.toNat, h⟩ v
+a.set ⟨i.toNat, h⟩ v
 
 /- "Comfortable" version of `fset`. It performs a bound check at runtime. -/
 @[extern c inline "lean_array_set(#2, #3, #4)"]
-def set (a : Array α) (i : @& Nat) (v : α) : Array α :=
-if h : i < a.size then a.fset ⟨i, h⟩ v else a
+def set! (a : Array α) (i : @& Nat) (v : α) : Array α :=
+if h : i < a.size then a.set ⟨i, h⟩ v else panic! "index out of bounds"
 
 @[extern c inline "lean_array_fswap(#2, #3, #4)"]
-def fswap (a : Array α) (i j : @& Fin a.size) : Array α :=
-let v₁ := a.fget i;
-let v₂ := a.fget j;
-let a  := a.fset i v₂;
-a.fset j v₁
+def swap (a : Array α) (i j : @& Fin a.size) : Array α :=
+let v₁ := a.get i;
+let v₂ := a.get j;
+let a  := a.set i v₂;
+a.set j v₁
 
 @[extern c inline "lean_array_swap(#2, #3, #4)"]
-def swap (a : Array α) (i j : @& Nat) : Array α :=
+def swap! (a : Array α) (i j : @& Nat) : Array α :=
 if h₁ : i < a.size then
-if h₂ : j < a.size then fswap a ⟨i, h₁⟩ ⟨j, h₂⟩
-else a
-else a
+if h₂ : j < a.size then swap a ⟨i, h₁⟩ ⟨j, h₂⟩
+else panic! "index out of bounds"
+else panic! "index out of bounds"
 
-@[inline] def fswapAt {α : Type} (a : Array α) (i : Fin a.size) (v : α) : α × Array α :=
-let e := a.fget i;
-let a := a.fset i v;
+@[inline] def swapAt {α : Type} (a : Array α) (i : Fin a.size) (v : α) : α × Array α :=
+let e := a.get i;
+let a := a.set i v;
 (e, a)
 
-@[inline] def swapAt {α : Type} (a : Array α) (i : Nat) (v : α) : α × Array α :=
-if h : i < a.size then fswapAt a ⟨i, h⟩ v else (v, a)
+-- TODO: delete as soon as we can define local instances
+@[neverExtract] private def swapAtPanic! [Inhabited α] (i : Nat) : α × Array α :=
+panic! ("index " ++ toString i ++ " out of bounds")
+
+@[inline] def swapAt! {α : Type} (a : Array α) (i : Nat) (v : α) : α × Array α :=
+if h : i < a.size then swapAt a ⟨i, h⟩ v else @swapAtPanic! _ ⟨v⟩ i
 
 @[extern c inline "lean_array_pop(#2)"]
 def pop (a : Array α) : Array α :=
 { sz   := Nat.pred a.size,
-  data := fun ⟨j, h⟩ => a.fget ⟨j, Nat.ltOfLtOfLe h (Nat.predLe _)⟩ }
+  data := fun ⟨j, h⟩ => a.get ⟨j, Nat.ltOfLtOfLe h (Nat.predLe _)⟩ }
 
 -- TODO(Leo): justify termination using wf-rec
 partial def shrink : Array α → Nat → Array α
@@ -149,7 +153,7 @@ variables {β : Type v} {σ : Type u}
 | i, b =>
   if h : i < a.size then
      let idx : Fin a.size := ⟨i, h⟩;
-     f idx (a.fget idx) b >>= miterateAux (i+1)
+     f idx (a.get idx) b >>= miterateAux (i+1)
   else pure b
 
 @[inline] def miterate (a : Array α) (b : β) (f : ∀ (i : Fin a.size), α → β → m β) : m β :=
@@ -168,7 +172,7 @@ miterateAux a (fun _ b a => f a b) ini b
      let idx₁ : Fin a₁.size := ⟨i, h₁⟩;
      if h₂ : i < a₂.size then
        let idx₂ : Fin a₂.size := ⟨i, h₂⟩;
-       f idx₁ (a₁.fget idx₁) (a₂.fget idx₂) b >>= miterate₂Aux (i+1)
+       f idx₁ (a₁.get idx₁) (a₂.get idx₂) b >>= miterate₂Aux (i+1)
      else pure b
   else pure b
 
@@ -184,7 +188,7 @@ miterate₂ a₁ a₂ b (fun _ a₁ a₂ b => f b a₁ a₂)
 | i =>
   if h : i < a.size then
      let idx : Fin a.size := ⟨i, h⟩;
-     do r ← f (a.fget idx);
+     do r ← f (a.get idx);
         match r with
         | some v => pure r
         | none   => mfindAux (i+1)
@@ -200,7 +204,7 @@ mfindAux a f 0
     have i - 1 < a.size from Nat.ltOfLtOfLe this h;
     let idx : Fin a.size := ⟨i - 1, this⟩;
     do
-      r ← f (a.fget idx);
+      r ← f (a.get idx);
       match r with
       | some v => pure r
       | none   =>
@@ -248,7 +252,7 @@ variables {m : Type → Type w} [Monad m]
 | i =>
   if h : i < a.size then
      let idx : Fin a.size := ⟨i, h⟩;
-     do b ← p (a.fget idx);
+     do b ← p (a.get idx);
      match b with
      | true  => pure true
      | false => anyMAux (i+1)
@@ -275,7 +279,7 @@ variable {β : Type v}
 | 0,   h, b => pure b
 | j+1, h, b => do
   let i : Fin a.size := ⟨j, h⟩;
-  b ← f i (a.fget i) b;
+  b ← f i (a.get i) b;
   miterateRevAux j (Nat.leOfLt h) b
 
 @[inline] def miterateRev (a : Array α) (b : β) (f : ∀ (i : Fin a.size), α → β → m β) : m β :=
@@ -309,9 +313,9 @@ variable {β:Type u}
 | i, a =>
   if h : i < a.size then
      let idx : Fin a.size := ⟨i, h⟩;
-     let v   : α          := a.fget idx;
-     let a                := a.fset idx (@unsafeCast _ _ ⟨v⟩ ());
-     do newV ← f i v; ummapAux (i+1) (a.fset idx (@unsafeCast _ _ ⟨v⟩ newV))
+     let v   : α          := a.get idx;
+     let a                := a.set idx (@unsafeCast _ _ ⟨v⟩ ());
+     do newV ← f i v; ummapAux (i+1) (a.set idx (@unsafeCast _ _ ⟨v⟩ newV))
   else
      pure (unsafeCast a)
 
@@ -334,10 +338,10 @@ variable {β:Type u}
 @[inline] def modify [Inhabited α] (a : Array α) (i : Nat) (f : α → α) : Array α :=
 if h : i < a.size then
   let idx : Fin a.size := ⟨i, h⟩;
-  let v                := a.fget idx;
-  let a                := a.fset idx (default α);
+  let v                := a.get idx;
+  let a                := a.set idx (arbitrary α);
   let v                := f v;
-  a.fset idx v
+  a.set idx v
 else
   a
 
@@ -357,7 +361,7 @@ partial def mforAux {α : Type w} {β : Type u} (f : α → m β) (a : Array α)
 | i =>
   if h : i < a.size then
      let idx : Fin a.size := ⟨i, h⟩;
-     let v   : α          := a.fget idx;
+     let v   : α          := a.get idx;
      f v *> mforAux (i+1)
   else
      pure ⟨⟩
@@ -372,7 +376,7 @@ partial def extractAux (a : Array α) : Nat → ∀ (e : Nat), e ≤ a.size → 
 | i, e, hle, r =>
   if hlt : i < e then
     let idx : Fin a.size := ⟨i, Nat.ltOfLtOfLe hlt hle⟩;
-    extractAux (i+1) e hle (r.push (a.fget idx))
+    extractAux (i+1) e hle (r.push (a.get idx))
  else r
 
 def extract (a : Array α) (b e : Nat) : Array α :=
@@ -391,7 +395,7 @@ partial def isEqvAux (a b : Array α) (hsz : a.size = b.size) (p : α → α →
   if h : i < a.size then
      let aidx : Fin a.size := ⟨i, h⟩;
      let bidx : Fin b.size := ⟨i, hsz ▸ h⟩;
-     match p (a.fget aidx) (b.fget bidx) with
+     match p (a.get aidx) (b.get bidx) with
      | true  => isEqvAux (i+1)
      | false => false
   else
@@ -411,7 +415,7 @@ partial def reverseAux : Array α → Nat → Array α
 | a, i =>
   let n := a.size;
   if i < n / 2 then
-    reverseAux (a.swap i (n - i - 1)) (i+1)
+    reverseAux (a.swap! i (n - i - 1)) (i+1)
   else
     a
 
@@ -422,9 +426,9 @@ reverseAux a 0
 @[specialize] partial def filterAux (p : α → Bool) : Array α → Nat → Nat → Array α
 | a, i, j =>
   if h₁ : i < a.size then
-    if p (a.fget ⟨i, h₁⟩) then
+    if p (a.get ⟨i, h₁⟩) then
        if h₂ : j < i then
-         filterAux (a.fswap ⟨i, h₁⟩ ⟨j, Nat.ltTrans h₂ h₁⟩) (i+1) (j+1)
+         filterAux (a.swap ⟨i, h₁⟩ ⟨j, Nat.ltTrans h₂ h₁⟩) (i+1) (j+1)
        else
          filterAux a (i+1) (j+1)
     else
@@ -439,7 +443,7 @@ partial def indexOfAux {α} [HasBeq α] (a : Array α) (v : α) : Nat → Option
 | i =>
   if h : i < a.size then
     let idx : Fin a.size := ⟨i, h⟩;
-    if a.fget idx == v then some idx
+    if a.get idx == v then some idx
     else indexOfAux (i+1)
   else none
 
@@ -451,7 +455,7 @@ partial def eraseIdxAux {α} : Nat → Array α → Array α
   if h : i < a.size then
     let idx  : Fin a.size := ⟨i, h⟩;
     let idx1 : Fin a.size := ⟨i - 1, Nat.ltOfLeOfLt (Nat.predLe i) h⟩;
-    eraseIdxAux (i+1) (a.fswap idx idx1)
+    eraseIdxAux (i+1) (a.swap idx idx1)
   else
     a.pop
 
@@ -461,7 +465,7 @@ eraseIdxAux (i.val + 1) a
 def eraseIdx {α} (a : Array α) (i : Nat) : Array α :=
 if i < a.size then eraseIdxAux (i+1) a else a
 
-theorem szFSwapEq (a : Array α) (i j : Fin a.size) : (a.fswap i j).size = a.size :=
+theorem szFSwapEq (a : Array α) (i j : Fin a.size) : (a.swap i j).size = a.size :=
 rfl
 
 theorem szPopEq (a : Array α) : a.pop.size = a.size - 1 :=
@@ -478,7 +482,7 @@ partial def eraseIdxSzAux {α} (a : Array α) : ∀ (i : Nat) (r : Array α), r.
   if h : i < r.size then
     let idx  : Fin r.size := ⟨i, h⟩;
     let idx1 : Fin r.size := ⟨i - 1, Nat.ltOfLeOfLt (Nat.predLe i) h⟩;
-    eraseIdxSzAux (i+1) (r.fswap idx idx1) ((szFSwapEq r idx idx1).trans heq)
+    eraseIdxSzAux (i+1) (r.swap idx idx1) ((szFSwapEq r idx idx1).trans heq)
   else
     ⟨r.pop, (szPopEq r).trans (heq ▸ rfl)⟩
 end
