tests/compiler/bytearray_bug.lean
@@ -1,4 +1,4 @@
 def main (xs : List String) : IO Unit :=
   let arr := (let e := ByteArray.empty; e.push (UInt8.ofNat 10));
-  let v := arr.data.get 0;
+  let v := arr.data.get! 0;
   IO.println v
