tests/lean/bytearray.lean
@@ -3,9 +3,9 @@ do
 let bs := [1, 2, 3].toByteArray;
 IO.println bs;
 let bs := bs.push 4;
-let bs := bs.set 1 20;
+let bs := bs.set! 1 20;
 IO.println bs;
-let bs₁ := bs.set 2 30;
+let bs₁ := bs.set! 2 30;
 IO.println bs₁;
 IO.println bs;
 IO.println bs.size;
