tests/lean/repr_issue.lean
@@ -1,7 +1,7 @@
 def foo {m} [Monad m] [MonadExcept String m] [MonadState (Array Nat) m] : m Nat :=
-catch (do modify $ fun (a : Array Nat) => a.set 0 33;
+catch (do modify $ fun (a : Array Nat) => a.set! 0 33;
           throw "error")
-      (fun _ => do a ← get; pure $ a.get 0)
+      (fun _ => do a ← get; pure $ a.get! 0)
 
 def ex₁ : StateT (Array Nat) (ExceptT String Id) Nat :=
 foo
